cleanup

code/poly1305/Hacl.Spec.Poly1305.Equiv.fst
@@ -23,11 +23,13 @@ val poly_update_repeat_blocks_multi_lemma:
   Lemma
     (normalize_n #w (repeat_blocks_multi #uint8 #(elem w) (w * size_block) text (poly1305_update_nblocks #w (compute_rw #w r)) acc) r ==
       repeat_blocks_multi #uint8 #pfelem size_block text (S.poly1305_update1 r size_block) (normalize_n #w acc r))
+
 let poly_update_repeat_blocks_multi_lemma #w text acc r =
   match w with
   | 1 -> Lemmas.poly_update_repeat_blocks_multi_lemma1 text acc r
   | 2 -> Lemmas.poly_update_repeat_blocks_multi_lemma2 text acc r
   | 4 -> Lemmas.poly_update_repeat_blocks_multi_lemma4 text acc r
+
 
 val poly_update_multi_lemma_load:
     #w:lanes
@@ -38,136 +40,13 @@ val poly_update_multi_lemma_load:
    (let t0 = Seq.slice text 0 (w * size_block) in
     normalize_n #w (load_acc #w acc0 t0) r ==
       repeat_blocks_multi #uint8 #pfelem size_block t0 (S.poly1305_update1 r size_block) acc0)
+
 let poly_update_multi_lemma_load #w text acc0 r =
   match w with
   | 1 -> Lemmas.poly_update_multi_lemma_load1 text acc0 r
   | 2 -> Lemmas.poly_update_multi_lemma_load2 text acc0 r
   | 4 -> Lemmas.poly_update_multi_lemma_load4 text acc0 r
 
-//
-// Lemma
-//   (poly_update_multi #w text acc0 r ==
-//      repeat_blocks_multi #uint8 #pfelem size_block text (update1 r size_block) acc0)
-//
-
-val poly_update_multi_lemma1:
-    #w:lanes
-  -> text:bytes{0 < length text /\ length text % (w * size_block) = 0}
-  -> acc0:pfelem
-  -> r:pfelem ->
-  Lemma
-   (let rw = compute_rw #w r in
-    let len = length text in
-    let len0 = w * size_block in
-    let t0 = Seq.slice text 0 len0 in
-    let f = S.poly1305_update1 r size_block in
-    let repeat_bf_t0 = repeat_blocks_f size_block text f (len / size_block) in
-    normalize_n #w (load_acc #w acc0 t0) r ==
-      Loops.repeat_right 0 (len0 / size_block) (Loops.fixed_a pfelem) repeat_bf_t0 acc0)
-let poly_update_multi_lemma1 #w text acc0 r =
-  let rw = compute_rw #w r in
-  let len = length text in
-  let len0 = w * size_block in
-  let t0 = Seq.slice text 0 len0 in
-  FStar.Seq.Base.lemma_len_slice text 0 len0;
-
-  let f = S.poly1305_update1 r size_block in
-  let repeat_bf_s0 = repeat_blocks_f size_block t0 f (len0 / size_block) in
-  let repeat_bf_t0 = repeat_blocks_f size_block text f (len / size_block) in
-
-  let aux_repeat_bf (i:nat{i < len0 / size_block}) (acc:pfelem) : Lemma
-    (repeat_bf_s0 i acc == repeat_bf_t0 i acc)
-    = let nb = len0 / size_block in
-      assert ((i+1) * size_block <= nb * size_block);
-      let block = Seq.slice text (i*size_block) (i*size_block+size_block) in
-      FStar.Seq.lemma_len_slice text (i*size_block) (i*size_block+size_block);
-      assert (repeat_bf_s0 i acc == f block acc);
-      assert (repeat_bf_t0 i acc == f block acc)
-  in
-
-  let acc1 = load_acc #w acc0 t0 in
-  poly_update_multi_lemma_load #w text acc0 r;
-  //assert (normalize_n #w acc1 r == repeat_blocks_multi #uint8 #pfelem size_block t0 (S.poly1305_update1 r size_block) acc0);
-  lemma_repeat_blocks_multi #uint8 #pfelem size_block t0 (S.poly1305_update1 r size_block) acc0;
-  //assert (normalize_n #w acc1 r == Loops.repeati (len0 / size_block) repeat_bf_s0 acc0);
-
-  FStar.Classical.forall_intro_2 (aux_repeat_bf);
-  PLoops.repeati_extensionality #pfelem (len0 / size_block) repeat_bf_s0 repeat_bf_t0 acc0;
-  assert (Loops.repeati (len0 / size_block) repeat_bf_s0 acc0 == Loops.repeati (len0 / size_block) repeat_bf_t0 acc0);
-
-  assert (normalize_n #w acc1 r == Loops.repeati (len0 / size_block) repeat_bf_t0 acc0);
-  Loops.repeati_def (len0 / size_block) repeat_bf_t0 acc0
-
-val poly_update_multi_lemma2:
-    #w:lanes
-  -> text:bytes{0 < length text /\ length text % (w * size_block) = 0}
-  -> acc0:pfelem
-  -> r:pfelem ->
-  Lemma
-   (let rw = compute_rw #w r in
-    let len = length text in
-    let len0 = w * size_block in
-    let t0 = Seq.slice text 0 len0 in
-    let t1 = Seq.slice text len0 len in
-    let f = S.poly1305_update1 r size_block in
-    let repeat_bf_t1 = repeat_blocks_f size_block text f (len / size_block) in
-
-    let acc1 = load_acc #w acc0 t0 in
-    let acc2 = repeat_blocks_multi #uint8 #(elem w) (w * size_block) t1 (poly1305_update_nblocks #w rw) acc1 in
-    normalize_n #w acc2 r ==
-      Loops.repeat_right (len0 / size_block) (len / size_block)
-        (Loops.fixed_a pfelem) repeat_bf_t1 (normalize_n #w acc1 r))
-let poly_update_multi_lemma2 #w text acc0 r =
-  let rw = compute_rw #w r in
-  let len = length text in
-  let len0 = w * size_block in
-  let len1 = len - len0 in
-  let t0 = Seq.slice text 0 len0 in
-  FStar.Seq.Base.lemma_len_slice text 0 len0;
-  let t1 = Seq.slice text len0 len in
-  FStar.Seq.Base.lemma_len_slice text len0 len;
-
-  let f = S.poly1305_update1 r size_block in
-  let repeat_bf_s1 = repeat_blocks_f size_block t1 f (len1 / size_block) in
-  let repeat_bf_t1 = repeat_blocks_f size_block text f (len / size_block) in
-
-  let i_start = len0 / size_block in
-  let nb = len1 / size_block in
-  assert (i_start + nb = len / size_block);
-
-  let aux_repeat_bf (i:nat{i < nb}) (acc:pfelem) : Lemma
-    (repeat_bf_s1 i acc == repeat_bf_t1 (i_start + i) acc)
-    =
-      let start = i_start * size_block in
-      assert (start + (i+1) * size_block <= start + nb * size_block);
-      let block = Seq.slice text (start+i*size_block) (start+i*size_block+size_block) in
-      FStar.Seq.lemma_len_slice text (start+i*size_block) (start+i*size_block+size_block);
-      assert (repeat_bf_s1 i acc == f block acc);
-      assert (repeat_bf_t1 (len0 / size_block + i) acc == f block acc)
-  in
-
-  let acc1 = load_acc #w acc0 t0 in
-  let acc2 = repeat_blocks_multi #uint8 #(elem w) (w * size_block) t1 (poly1305_update_nblocks #w rw) acc1 in
-  let acc3 = normalize_n #w acc2 r in
-  assert (acc3 == poly1305_update_multi #w text acc0 r);
-  poly_update_repeat_blocks_multi_lemma #w t1 acc1 r;
-  //assert (acc3 == repeat_blocks_multi #uint8 #pfelem size_block t1 (S.poly1305_update1 r size_block) (normalize_n #w acc1 r));
-  lemma_repeat_blocks_multi #uint8 #pfelem size_block t1 (S.poly1305_update1 r size_block) (normalize_n #w acc1 r);
-  //assert (acc3 == Loops.repeati (len1 / size_block) repeat_bf_s1 (normalize_n #w acc1 r));
-  let acc1_s = normalize_n #w acc1 r in
-  Loops.repeati_def (len1 / size_block) repeat_bf_s1 acc1_s;
-  //assert (acc3 == Loops.repeat_right 0 (len1 / size_block) (Loops.fixed_a pfelem) repeat_bf_s1 acc1_s);
-
-  FStar.Classical.forall_intro_2 (aux_repeat_bf);
-  PLoops.repeati_right_extensionality nb i_start (nb+i_start) repeat_bf_s1 repeat_bf_t1 acc1_s;
-  assert (
-    Loops.repeat_right 0 nb (Loops.fixed_a pfelem) repeat_bf_s1 acc1_s ==
-    Loops.repeat_right i_start (i_start+nb) (Loops.fixed_a pfelem) repeat_bf_t1 acc1_s);
-
-  assert (acc3 ==
-    Loops.repeat_right (len0 / size_block) (len / size_block)
-    (Loops.fixed_a pfelem)
-    repeat_bf_t1 acc1_s)
 
 val poly_update_multi_lemma:
     #w:lanes
@@ -177,47 +56,29 @@ val poly_update_multi_lemma:
     Lemma
     (poly1305_update_multi #w text acc0 r ==
       repeat_blocks_multi #uint8 #pfelem size_block text (S.poly1305_update1 r size_block) acc0)
+
 let poly_update_multi_lemma #w text acc0 r =
   let rw = compute_rw #w r in
   let len = length text in
+  let len0 = w * size_block in
+
+  let t0 = Seq.slice text 0 len0 in
+  let t1 = Seq.slice text len0 len in
+
   let f = S.poly1305_update1 r size_block in
   let repeat_bf_t0 = repeat_blocks_f size_block text f (len / size_block) in
-
-  let len0 = w * size_block in
-  let t0 = Seq.slice text 0 len0 in
-  FStar.Seq.Base.lemma_len_slice text 0 len0;
-  let t1 = Seq.slice text len0 len in
-  FStar.Seq.Base.lemma_len_slice text len0 len;
 
   let acc1 = load_acc #w acc0 t0 in
   let acc2 = repeat_blocks_multi #uint8 #(elem w) (w * size_block) t1 (poly1305_update_nblocks #w rw) acc1 in
   let acc3 = normalize_n #w acc2 r in
   assert (acc3 == poly1305_update_multi #w text acc0 r);
   poly_update_repeat_blocks_multi_lemma #w t1 acc1 r;
-  assert (acc3 == repeat_blocks_multi #uint8 #pfelem size_block t1 (S.poly1305_update1 r size_block) (normalize_n acc1 r));
-  poly_update_multi_lemma2 #w text acc0 r;
-  assert (acc3 ==
-   Loops.repeat_right (len0 / size_block) (len / size_block)
-     (Loops.fixed_a pfelem) repeat_bf_t0 (normalize_n #w acc1 r));
+  assert (acc3 == repeat_blocks_multi #uint8 #pfelem size_block t1 f (normalize_n acc1 r));
 
-  poly_update_multi_lemma1 #w text acc0 r;
+  poly_update_multi_lemma_load #w text acc0 r;
+  assert (normalize_n acc1 r == repeat_blocks_multi #uint8 #pfelem size_block t0 f acc0);
+  PLoops.repeat_blocks_multi_split #uint8 #pfelem size_block len0 text f acc0
 
-  Loops.repeat_right_plus
-    0 (len0 / size_block) (len / size_block)
-    (Loops.fixed_a pfelem)
-    repeat_bf_t0 acc0;
-  assert (acc3 ==
-    Loops.repeat_right 0 (len / size_block)
-    (Loops.fixed_a pfelem)
-    repeat_bf_t0 acc0);
-  Loops.repeati_def (len / size_block) repeat_bf_t0 acc0;
-  lemma_repeat_blocks_multi #uint8 #pfelem size_block text (S.poly1305_update1 r size_block) acc0;
-  assert (acc3 == repeat_blocks_multi #uint8 #pfelem size_block text (S.poly1305_update1 r size_block) acc0)
-
-//
-// Lemma
-//   (poly #w text acc0 r == S.poly1305_update1 text acc0 r)
-//
 
 val poly_eq_lemma:
     #w:lanes
